Update Equiv_J.v

Equiv_J.v
@@ -1,7 +1,6 @@
-(** * Equiv_J: プログラムの同値性 *)
 (* * Equiv: Program Equivalence *)
+(** * Equiv_J: プログラムの同値性 *)
 
-(* $Date: 2011-04-05 21:37:47 -0400 (Tue, 05 Apr 2011) $ *)
 
 
 Require Export Imp_J.
@@ -55,7 +54,6 @@ Require Export Imp_J.
     simple program transformation: the [optimize_0plus] function.  The
     programming language we were considering was the first version of
     the language of arithmetic expressions -- with no variables -- so
-
     in that setting it was very easy to define what it _means_ for a
     program transformation to be correct: it should always yield a
     program that evaluates to the same number as the original.  
@@ -86,7 +84,7 @@ Require Export Imp_J.
 (** 変数を伴う[aexp]と[bexp]については、どう定義すれば良いかは明らかです。
     2つの[aexp]または[bexp]が振る舞い同値である(_behaviorally equivalent_)とは、
     「すべての状態で」2つの評価結果が同じになることです。*)    
-
+ 
 Definition aequiv (a1 a2 : aexp) : Prop :=
   forall (st:state), 
     aeval st a1 = aeval st a2.
@@ -120,74 +118,81 @@ Definition cequiv (c1 c2 : com) : Prop :=
   forall (st st' : state), 
     (c1 / st || st') <-> (c2 / st || st').
 
-(* **** Exercise: 2 stars, optional (pairs_equiv) *)
-(** **** 練習問題: ★★, optional (pairs_equiv) *)
-(* Which of the following pairs of programs are equivalent? Write
-    "yes" or "no" for each one.
 
-(a)
-[[
-    WHILE (BLe (ANum 1) (AId X)) DO
-      X ::= APlus (AId X) (ANum 1)
-    END
-]]
-    and
-[[
-    WHILE (BLe (ANum 2) (AId X)) DO
-      X ::= APlus (AId X) (ANum 1)
-    END
-]]
-(* FILL IN HERE *)
 
-(b)
-[[
-    WHILE BTrue DO
-      WHILE BFalse DO X ::= APlus (AId X) (ANum 1) END
-    END
-]]
-and
-[[
-    WHILE BFalse DO
-      WHILE BTrue DO X ::= APlus (AId X) (ANum 1) END
-    END
-]]
+(*  **** Exercise: 2 stars (equiv_classes)  *)
+(** **** 練習問題: ★★, (equiv_classes) *)
 
-(* FILL IN HERE *)
+(*  Given the following programs, group together those that are
+    equivalent in [Imp]. Your answer should be given as a list of
+    lists, where each sub-list represents a group of equivalent
+    programs. For example, if you think programs (a) through (h) are
+    all equivalent to each other, but not to (i), your answer should
+    look like this:
 
-[] *)
-(** 以下のプログラムの対の中で、同値なのはどれでしょうか？
-    それぞれについて、"yes" か "no" を書きなさい。
+    [ [prog_a;prog_b;prog_c;prog_d;prog_e;prog_f;prog_g;prog_h] ;
+      [prog_i] ]
 
-(a)
-[[
-    WHILE (BLe (ANum 1) (AId X)) DO
-      X ::= APlus (AId X) (ANum 1)
-    END
-]]
-    と
-[[
-    WHILE (BLe (ANum 2) (AId X)) DO
-      X ::= APlus (AId X) (ANum 1)
-    END
-]]
-(* FILL IN HERE *)
+    Write down your answer below in the definition of [equiv_classes]. *)
+(** 次のプログラムが与えられたとき、[Imp]において等しいものグループを作りなさい。
+    あなたの答をリストのリストとして表現し、それぞれのサブリストが等価なプログラムのグループを表すようにしなさい。例えば、(a)から(h)までが全て同じプログラムであり、(i)だけが違うと思うならば、答は次のようになります：
 
-(b)
-[[
-    WHILE BTrue DO
-      WHILE BFalse DO X ::= APlus (AId X) (ANum 1) END
-    END
-]]
-    と
-[[
-    WHILE BFalse DO
-      WHILE BTrue DO X ::= APlus (AId X) (ANum 1) END
-    END
-]]
+    [ [prog_a;prog_b;prog_c;prog_d;prog_e;prog_f;prog_g;prog_h] ;
+      [prog_i] ]
 
-(* FILL IN HERE *)
+    あなたの答えを[equiv_classes]という名前で定義しなさい。*)
 
-[] *)
+Definition prog_a : com :=
+  WHILE BNot (BLe (AId X) (ANum 0)) DO
+    X ::= APlus (AId X) (ANum 1)
+  END.
+
+Definition prog_b : com :=
+  IFB BEq (AId X) (ANum 0) THEN
+    X ::= APlus (AId X) (ANum 1);;
+    Y ::= ANum 1
+  ELSE
+    Y ::= ANum 0
+  FI;;
+  X ::= AMinus (AId X) (AId Y);;
+  Y ::= ANum 0.
+
+Definition prog_c : com :=
+  SKIP.
+
+Definition prog_d : com :=
+  WHILE BNot (BEq (AId X) (ANum 0)) DO
+    X ::= APlus (AMult (AId X) (AId Y)) (ANum 1)
+  END.
+
+Definition prog_e : com :=
+  Y ::= ANum 0.
+
+Definition prog_f : com :=
+  Y ::= APlus (AId X) (ANum 1);;
+  WHILE BNot (BEq (AId X) (AId Y)) DO
+    Y ::= APlus (AId X) (ANum 1)
+  END.
+
+Definition prog_g : com :=
+  WHILE BTrue DO
+    SKIP
+  END.
+
+Definition prog_h : com :=
+  WHILE BNot (BEq (AId X) (AId X)) DO
+    X ::= APlus (AId X) (ANum 1)
+  END.
+
+Definition prog_i : com :=
+  WHILE BNot (BEq (AId X) (AId Y)) DO
+    X ::= APlus (AId Y) (ANum 1)
+  END.
+
+Definition equiv_classes : list (list com) :=
+(* FILL IN HERE *) admit.
+(* GRADE_TEST 2: check_equiv_classes equiv_classes *)
+(** [] *)
 
 (* ####################################################### *)
 (* ** Examples *)
@@ -195,7 +200,6 @@ and
 
 (*  Here are some simple examples of equivalences of arithmetic
     and boolean expressions. *)
-(** 
 
 Theorem aequiv_example:
   aequiv (AMinus (AId X) (AId X)) (ANum 0).
@@ -237,41 +241,49 @@ Qed.
 (** **** 練習問題: ★★ (skip_right) *)
 (*  Prove that adding a SKIP after a command results in an equivalent
     program *)
-(**
-*)
+(** SKIPをコマンドの結果の後ろに追加することはもとのプログラムと等しいことを証明しなさい *)
+
 
 Theorem skip_right: forall c,
-  cequiv
-    (c; SKIP)
+  cequiv 
+    (c;; SKIP) 
     c.
-Proof.
+Proof. 
   (* FILL IN HERE *) Admitted.
 (** [] *)
 
-(* We can also explore transformations that simplify [IFB]
+(** Similarly, here is a simple transformations that simplifies [IFB]
     commands: *)
-(** [IFB]コマンドを簡単化する変換を探索することもできます: *)
+(** 同様に[IFB]コマンドを簡単化する単純な変換です: *)
 
 Theorem IFB_true_simple: forall c1 c2,
-  cequiv
-    (IFB BTrue THEN c1 ELSE c2 FI)
+  cequiv 
+    (IFB BTrue THEN c1 ELSE c2 FI) 
     c1.
-Proof.
-  intros c1 c2.
+Proof. 
+  intros c1 c2. 
   split; intros H.
   Case "->".
     inversion H; subst. assumption. inversion H5.
   Case "<-".
     apply E_IfTrue. reflexivity. assumption.  Qed.
 
-(* Of course, few programmers would be tempted to write a conditional
+
+(*  Of course, few programmers would be tempted to write a conditional
     whose guard is literally [BTrue].  A more interesting case is when
-    the guard is _equivalent_ to true...
+    the guard is _equivalent_ to true:
 
    _Theorem_: If [b] is equivalent to [BTrue], then [IFB b THEN c1
    ELSE c2 FI] is equivalent to [c1].
+*)
+(** もちろん、ガードが[BTrue]そのままである条件文を書こうとするプログラマはほとんどいないでしょう。
+    より興味深いのは、ガードが真と「同値である」場合です:
 
-   _Proof_:
+   「定理」:もし[b]が[BTrue]と同値ならば、[IFB b THEN c1 ELSE c2 FI]は[c1]と同値である。
+*)
+(** *** *)
+(**
+   _Proof_: 
 
      - ([->]) We must show, for all [st] and [st'], that if [IFB b
        THEN c1 ELSE c2 FI / st || st'] then [c1 / st || st'].
@@ -305,11 +317,7 @@ Proof.
        c1 ELSE c2 FI / st || st'].  []
 
    Here is the formal version of this proof: *)
-(** もちろん、ガードが[BTrue]そのままである条件文を書こうとするプログラマはほとんどいないでしょう。
-    より興味深いのは、ガードが真と「同値である」場合です...
-
-   「定理」:もし[b]が[BTrue]と同値ならば、[IFB b THEN c1 ELSE c2 FI]は[c1]と同値である。
-
+(** 
    「証明」:
 
      - ([->]) すべての[st]と[st']に対して、もし[IFB b THEN c1 ELSE c2 FI / st || st']
@@ -348,8 +356,8 @@ Proof.
 
 Theorem IFB_true: forall b c1 c2,
      bequiv b BTrue  ->
-     cequiv
-       (IFB b THEN c1 ELSE c2 FI)
+     cequiv 
+       (IFB b THEN c1 ELSE c2 FI) 
        c1.
 Proof.
   intros b c1 c2 Hb.
@@ -359,30 +367,30 @@ Proof.
     SCase "b evaluates to true".
       assumption.
     SCase "b evaluates to false (contradiction)".
+      unfold bequiv in Hb. simpl in Hb.
       rewrite Hb in H5.
       inversion H5.
   Case "<-".
     apply E_IfTrue; try assumption.
+    unfold bequiv in Hb. simpl in Hb.
     rewrite Hb. reflexivity.  Qed.
 
-(* **** Exercise: 2 stars, recommended (IFB_false) *)
-(** **** 練習問題: ★★, recommended (IFB_false) *)
+(*  **** Exercise: 2 stars (IFB_false)  *)
+(** **** 練習問題: ★★ (IFB_false) *)
 Theorem IFB_false: forall b c1 c2,
   bequiv b BFalse  ->
-  cequiv
-    (IFB b THEN c1 ELSE c2 FI)
+  cequiv 
+    (IFB b THEN c1 ELSE c2 FI) 
     c2.
 Proof.
   (* FILL IN HERE *) Admitted.
 (** [] *)
 
-(* **** Exercise: 3 stars (swap_if_branches) *)
-(** **** 練習問題: ★★★ (swap_if_branches) *)
-(*  Show that we can swap the branches of an IF by negating its
+(* **** Exercise: 3 stars (swap_if_branches)  *)
+(** **** 練習問題: ★★ (swap_if_branches) *)
+(* Show that we can swap the branches of an IF by negating its
     condition *)
-(** *)
-
-
+(** IFの条件の枝が否定によって交換可能であることを示しなさい *)
 Theorem swap_if_branches: forall b e1 e2,
   cequiv
     (IFB b THEN e1 ELSE e2 FI)
@@ -391,12 +399,14 @@ Proof.
   (* FILL IN HERE *) Admitted.
 (** [] *)
 
-(* For while loops, there is a similar pair of theorems: a loop whose
-    guard is equivalent to [BFalse] is equivalent to [SKIP], while a
-    loop whose guard is equivalent to [BTrue] is equivalent to [WHILE
-    BTrue DO SKIP END] (or any other non-terminating program).  The
-    first of these facts is easy. *)
-(** whileループについては、同様の2つ定理があります:
+(** *** *)
+
+(*  For [WHILE] loops, we can give a similar pair of theorems.  A loop
+    whose guard is equivalent to [BFalse] is equivalent to [SKIP],
+    while a loop whose guard is equivalent to [BTrue] is equivalent to
+    [WHILE BTrue DO SKIP END] (or any other non-terminating program).
+    The first of these facts is easy. *)
+(** [WHILE]ループについては、同様の2つ定理があります:
     ガードが[BFalse]と同値であるループは[SKIP]と同値である、というものと、
     ガードが[BTrue]と同値であるループは[WHILE BTrue DO SKIP END]
     (あるいは他の任意の停止しないプログラム)と同値である、というものです。
@@ -407,7 +417,7 @@ Theorem WHILE_false : forall b c,
      cequiv
        (WHILE b DO c END)
        SKIP.
-Proof.
+Proof. 
   intros b c Hb. split; intros H.
   Case "->".
     inversion H; subst.
@@ -443,7 +453,7 @@ Proof.
 
     _Proof_: Suppose that [(WHILE b DO c END) / st || st'].  We show,
     by induction on a derivation of [(WHILE b DO c END) / st || st'],
-    that this assumption leads to a contradiction.
+    that this assumption leads to a contradiction.  
 
       - Suppose [(WHILE b DO c END) / st || st'] is proved using rule
         [E_WhileEnd].  Then by assumption [beval st b = false].  But
@@ -485,16 +495,19 @@ Proof.
 Lemma WHILE_true_nonterm : forall b c st st',
      bequiv b BTrue ->
      ~( (WHILE b DO c END) / st || st' ).
-Proof.
+Proof. 
+  (* WORKED IN CLASS *)
   intros b c st st' Hb.
   intros H.
-  remember (WHILE b DO c END) as cw.
+  remember (WHILE b DO c END) as cw eqn:Heqcw.
   ceval_cases (induction H) Case;
-    (* Most rules don't apply, and we can rule them out
+    (* Most rules don't apply, and we can rule them out 
        by inversion *)
     inversion Heqcw; subst; clear Heqcw.
-  (* The two interesting cases are the ones for while loops: *)
+  (* The two interesting cases are the ones for WHILE loops: *)
   Case "E_WhileEnd". (* contradictory -- b is always true! *)
+    unfold bequiv in Hb.
+    (* [rewrite] is able to instantiate the quantifier in [st] *)
     rewrite Hb in H. inversion H.
   Case "E_WhileLoop". (* immediate from the IH *)
     apply IHceval2. reflexivity.  Qed.
@@ -518,23 +531,23 @@ Proof.
 
 Theorem WHILE_true: forall b c,
      bequiv b BTrue  ->
-     cequiv
+     cequiv 
        (WHILE b DO c END)
        (WHILE BTrue DO SKIP END).
-Proof.
+Proof. 
   (* FILL IN HERE *) Admitted.
 (** [] *)
 
 Theorem loop_unrolling: forall b c,
   cequiv
     (WHILE b DO c END)
-    (IFB b THEN (c; WHILE b DO c END) ELSE SKIP FI).
+    (IFB b THEN (c;; WHILE b DO c END) ELSE SKIP FI).
 Proof.
   (* WORKED IN CLASS *)
   intros b c st st'.
   split; intros Hce.
   Case "->".
-    inversion Hce; subst.
+    inversion Hce; subst.  
     SCase "loop doesn't run".
       apply E_IfFalse. assumption. apply E_Skip.
     SCase "loop runs".
@@ -544,7 +557,7 @@ Proof.
     inversion Hce; subst.
     SCase "loop runs".
       inversion H5; subst.
-      apply E_WhileLoop with (st' := st'0).
+      apply E_WhileLoop with (st' := st'0). 
       assumption. assumption. assumption.
     SCase "loop doesn't run".
       inversion H5; subst. apply E_WhileEnd. assumption.  Qed.
@@ -552,81 +565,77 @@ Proof.
 (* **** Exercise: 2 stars, optional (seq_assoc) *)
 (** **** 練習問題: ★★, optional (seq_assoc) *)
 Theorem seq_assoc : forall c1 c2 c3,
-  cequiv ((c1;c2);c3) (c1;(c2;c3)).
+  cequiv ((c1;;c2);;c3) (c1;;(c2;;c3)).
 Proof.
   (* FILL IN HERE *) Admitted.
 (** [] *)
 
-(* Finally, let's look at simple equivalences involving assignments.
-    This turns out to be a little tricky.
-    To start with, we might expect to be able to show that certain
-    kinds of "useless" assignments can be removed. Most trivially: *)
+(*  ** The Functional Equivalence Axiom *)
+(** ** 関数の同値性の公理 *)
+
+(*  Finally, let's look at simple equivalences involving assignments.
+    For example, we might expect to be able to show that [X ::= AId X]
+    is equivalent to [SKIP].  However, when we try to show it, we get
+    stuck in an interesting way. *)
 (** 最後に、代入に関する簡単な同値を見てみましょう。
-    これは、ちょっとトリッキーです。
-    まず最初に、ある種の「意味のない」代入が除去できることを示せないか、やってみましょう。
-    一番自明なのは: *)
+    たとえば、[X ::= AId X]は、[SKIP]と同値であることを示すことが出来るかもしれないと思うかもしれません。しかしながら、それをやろうとすると簡単に行き詰まってしまいます。
+*)
 
 Theorem identity_assignment_first_try : forall (X:id),
-  cequiv
-    (X ::= AId X)
-    SKIP.
-Proof.
+  cequiv (X ::= AId X) SKIP.
+Proof. 
    intros. split; intro H.
-     Case "->".
+     Case "->". 
        inversion H; subst.  simpl.
-       replace (update st X (st X)) with st.
-       constructor.
-       (* But here we're stuck. The goal looks reasonable, but in fact
-          it is not provable!  If we look back at the set of lemmas we
-          proved about [update] in the last chapter, we can see that
-          lemma [update_same] almost does the job, but not quite: it
-          says that the original and updated states agree at all
-          values, but this is not the same thing as saying that they
-          are [eq] in Coq's sense! *)
-       (* しかしここで行き詰まります。ゴールは合理的に見えますが、しかし実は証明できません!
-          前の章で[update]に関して証明した補題のセットをふりかえってみましょう。
-          補題[update_same]がほとんどのことをやっていますが、全部ではありません。
-          [update_same]
-          は元の状態と更新された状態がすべての値について一致することを言っていますが、
-          それは、Coqの意味で[eq]だと言っているわけではありません! *)
-Admitted.
+       replace (update st X (st X)) with st.  
+       constructor. 
+       (* 詰った... *) Abort.
 
-(* What is going on here?  Recall that our states are just functions
-    from identifiers to values.  For Coq, functions are only equal
-    when their definitions are syntactically the same, modulo
+(*  Here we're stuck. The goal looks reasonable, but in fact it is not
+    provable!  If we look back at the set of lemmas we proved about
+    [update] in the last chapter, we can see that lemma [update_same]
+    almost does the job, but not quite: it says that the original and
+    updated states agree at all values, but this is not the same thing
+    as saying that they are [=] in Coq's sense! *)
+(** ここで行き詰まります。ゴールは合理的に見えますが、しかし実は証明できません!
+    前の章で[update]に関して証明した補題のセットをふりかえってみましょう。
+    補題[update_same]がほとんどのことをやっていますが、全部ではありません。
+    [update_same]は元の状態と更新された状態がすべての値について一致することを
+    言っていますが、
+    それは、Coqの意味で[eq]だと言っているわけではありません! *)
+
+(*  What is going on here?  Recall that our states are just
+    functions from identifiers to values.  For Coq, functions are only
+    equal when their definitions are syntactically the same, modulo
     simplification.  (This is the only way we can legally apply the
-    [eq] constructor!) In practice, for functions built up by repeated
-    uses of the [update] operation, this means that two functions can
-    be proven equal only if they were constructed using the _same_
-    [update] operations, applied in the same order.  In the theorem
-    above, the sequence of updates on the first parameter [cequiv] is
-    one longer than for the second parameter, so it is no wonder that
-    the equality doesn't hold.
+    [refl_equal] constructor of the inductively defined proposition
+    [eq]!) In practice, for functions built up by repeated uses of the
+    [update] operation, this means that two functions can be proven
+    equal only if they were constructed using the _same_ [update]
+    operations, applied in the same order.  In the theorem above, the
+    sequence of updates on the first parameter [cequiv] is one longer
+    than for the second parameter, so it is no wonder that the
+    equality doesn't hold. *)
 
-    But the problem is quite general. If we try to prove other
-    "trivial" facts, such as
-[[
-    cequiv (X ::= APlus (AId X ANum 1) ;
-            X ::= APlus (AId X ANum 1))
-           (X ::= APlus (AId X ANum 2))
-]]
+(** *** *)
+(** This problem is actually quite general. If we try to prove other
+    simple facts, such as
+    cequiv (X ::= X + 1;;
+            X ::= X + 1)
+           (X ::= X + 2)
     or
-[[
-    cequiv (X ::= ANum 1; Y ::= ANum 2)
-           (y ::= ANum 2; X ::= ANum 1)
-
-]]
+    cequiv (X ::= 1;; Y ::= 2)
+           (y ::= 2;; X ::= 1)
+  
     we'll get stuck in the same way: we'll have two functions that
     behave the same way on all inputs, but cannot be proven to be [eq]
     to each other.
 
     The reasoning principle we would like to use in these situations
     is called _functional extensionality_:
-[[[
                         forall x, f x = g x
                         -------------------
                                f = g
-]]]
     Although this principle is not derivable in Coq's built-in logic,
     it is safe to add it as an additional _axiom_.  *)
 (** 何がどうなっているのでしょう？
@@ -641,28 +650,22 @@ Admitted.
 
     しかし、この問題はかなり一般的なものです。
     何か別の「自明な」事実、例えば
-[[
-    cequiv (X ::= APlus (AId X ANum 1) ;
-            X ::= APlus (AId X ANum 1))
-           (X ::= APlus (AId X ANum 2))
-]]
+    cequiv (X ::= X + 1;;
+            X ::= X + 1)
+           (X ::= X + 2)
     あるいは
-[[
-    cequiv (X ::= ANum 1; Y ::= ANum 2)
-           (y ::= ANum 2; X ::= ANum 1)
+    cequiv (X ::= 1;; Y ::= 2)
+           (y ::= 2;; X ::= 1)
 
-]]
     を証明しようとするとき、同じように行き詰まることになります。
     つまり、すべての入力に対して同一の振る舞いをする2つの関数が出てくるのですが、
     その2つが[eq]であることが証明できないのです。
 
     こういった状況でこれから使おうとしている推論原理は、
     関数外延性(_functional extensionality_)と呼ばれます:
-[[
                         forall x, f x = g x
                         -------------------
                                f = g
-]]
     この原理は Coq のビルトインの論理からは導出できませんが、
     追加公理(_axiom_)として導入することは安全です。*)    
 
@@ -671,40 +674,39 @@ Axiom functional_extensionality : forall {X Y: Type} {f g : X -> Y},
 
 (* It can be shown that adding this axiom doesn't introduce any
     inconsistencies into Coq.  (In this way, it is similar to adding
-    one of the classical logic axioms, such as [excluded_middle].)
-
-    With the benefit of this axiom we can prove our theorem: *)
+    one of the classical logic axioms, such as [excluded_middle].) *)
 (** Coq にこの公理を導入することが矛盾を生むものではないことを示すことができます。
     (このように、この公理の導入は、
-     [excluded_middle]のような古典論理の公理を追加するのと同様なのです。)
+     [excluded_middle]のような古典論理の公理を追加するのと同様なのです。) *)
 
-    この公理のおかげで、先の定理を証明することができます: *)
+(*  With the benefit of this axiom we can prove our theorem.  *)
+(** この公理のおかげで、先の定理を証明することができます: *)
 
 Theorem identity_assignment : forall (X:id),
   cequiv
     (X ::= AId X)
     SKIP.
-Proof.
+Proof. 
    intros. split; intro H.
-     Case "->".
+     Case "->". 
        inversion H; subst. simpl.
-       replace (update st X (st X)) with st.
-       constructor.
-       apply functional_extensionality. intro.
-       rewrite update_same; reflexivity.
+       replace (update st X (st X)) with st.  
+       constructor. 
+       apply functional_extensionality. intro. 
+       rewrite update_same; reflexivity.  
      Case "<-".
-       inversion H; subst.
+       inversion H; subst. 
        assert (st' = (update st' X (st' X))).
-          apply functional_extensionality. intro.
+          apply functional_extensionality. intro. 
           rewrite update_same; reflexivity.
-       rewrite H0 at 2.
+       rewrite H0 at 2. 
        constructor. reflexivity.
 Qed.
 
-(* **** Exercise: 2 stars, recommended (assign_aequiv) *)
-(** **** 練習問題: ★★, recommended (assign_aequiv) *)
+(*  **** Exercise: 2 stars (assign_aequiv)  *)
+(** **** 練習問題: ★★ (assign_aequiv) *)
 Theorem assign_aequiv : forall X e,
-  aequiv (AId X) e ->
+  aequiv (AId X) e -> 
   cequiv SKIP (X ::= e).
 Proof.
   (* FILL IN HERE *) Admitted.
@@ -724,21 +726,21 @@ Proof.
 
 (* First, we verify that the equivalences on [aexps], [bexps], and
     [com]s really are _equivalences_ -- i.e., that they are reflexive,
-    symmetric, and transitive: *)
+    symmetric, and transitive.  The proofs are all easy. *)
 (** 最初に、[aexps]、[bexps]、[com]の同値が、本当に「同値関係」であること、つまり、
-    反射性、対称性、推移性を持つことを検証します: *)
+    反射性、対称性、推移性を持つことを検証します。証明はすべて簡単です。 *)
 
 Lemma refl_aequiv : forall (a : aexp), aequiv a a.
 Proof.
   intros a st. reflexivity.  Qed.
 
-Lemma sym_aequiv : forall (a1 a2 : aexp),
+Lemma sym_aequiv : forall (a1 a2 : aexp), 
   aequiv a1 a2 -> aequiv a2 a1.
 Proof.
   intros a1 a2 H. intros st. symmetry. apply H.  Qed.
 
-Lemma trans_aequiv : forall (a1 a2 a3 : aexp),
-  aequiv a1 a2 -> aequiv a2 a3 -> aequiv a1 a3.
+Lemma trans_aequiv : forall (a1 a2 a3 : aexp), 
+  aequiv a1 a2 -> aequiv a2 a3 -> aequiv a1 a3. 
 Proof.
   unfold aequiv. intros a1 a2 a3 H12 H23 st.
   rewrite (H12 st). rewrite (H23 st). reflexivity.  Qed.
@@ -747,13 +749,13 @@ Lemma refl_bequiv : forall (b : bexp), bequiv b b.
 Proof.
   unfold bequiv. intros b st. reflexivity.  Qed.
 
-Lemma sym_bequiv : forall (b1 b2 : bexp),
+Lemma sym_bequiv : forall (b1 b2 : bexp), 
   bequiv b1 b2 -> bequiv b2 b1.
 Proof.
   unfold bequiv. intros b1 b2 H. intros st. symmetry. apply H.  Qed.
 
-Lemma trans_bequiv : forall (b1 b2 b3 : bexp),
-  bequiv b1 b2 -> bequiv b2 b3 -> bequiv b1 b3.
+Lemma trans_bequiv : forall (b1 b2 b3 : bexp), 
+  bequiv b1 b2 -> bequiv b2 b3 -> bequiv b1 b3. 
 Proof.
   unfold bequiv. intros b1 b2 b3 H12 H23 st.
   rewrite (H12 st). rewrite (H23 st). reflexivity.  Qed.
@@ -762,60 +764,51 @@ Lemma refl_cequiv : forall (c : com), cequiv c c.
 Proof.
   unfold cequiv. intros c st st'. apply iff_refl.  Qed.
 
-Lemma sym_cequiv : forall (c1 c2 : com),
+Lemma sym_cequiv : forall (c1 c2 : com), 
   cequiv c1 c2 -> cequiv c2 c1.
 Proof.
   unfold cequiv. intros c1 c2 H st st'.
-  assert (c1 / st || st' <-> c2 / st || st') as H'.
+  assert (c1 / st || st' <-> c2 / st || st') as H'. 
     SCase "Proof of assertion". apply H.
   apply iff_sym. assumption.
 Qed.
 
-Lemma iff_trans : forall (P1 P2 P3 : Prop),
+Lemma iff_trans : forall (P1 P2 P3 : Prop), 
   (P1 <-> P2) -> (P2 <-> P3) -> (P1 <-> P3).
 Proof.
   intros P1 P2 P3 H12 H23.
   inversion H12. inversion H23.
-  split; intros A.
+  split; intros A. 
     apply H1. apply H. apply A.
     apply H0. apply H2. apply A.  Qed.
 
-Lemma trans_cequiv : forall (c1 c2 c3 : com),
-  cequiv c1 c2 -> cequiv c2 c3 -> cequiv c1 c3.
+Lemma trans_cequiv : forall (c1 c2 c3 : com), 
+  cequiv c1 c2 -> cequiv c2 c3 -> cequiv c1 c3. 
 Proof.
   unfold cequiv. intros c1 c2 c3 H12 H23 st st'.
   apply iff_trans with (c2 / st || st'). apply H12. apply H23.  Qed.
 
-(* ########################################################*)
+(* ######################################################## *)
 (* ** Behavioral Equivalence is a Congruence *)
 (** ** 振る舞い同値は合同関係である *)
 
 (* Less obviously, behavioral equivalence is also a _congruence_.
     That is, the equivalence of two subprograms implies the
-    equivalence of the whole programs in which they are embedded:
-[[[
+    equivalence of the larger programs in which they are embedded:
               aequiv a1 a1'
       -----------------------------
       cequiv (i ::= a1) (i ::= a1')
-
-              cequiv c1 c1'
+ 
+              cequiv c1 c1'    
               cequiv c2 c2'
          ------------------------
-         cequiv (c1;c2) (c1';c2')
-]]]
-    ...and so on.  (Note that we are using the inference rule notation
-    here not as part of a definition, but simply to write down some
-    valid implications in a readable format. We prove these
-    implications below.)
+         cequiv (c1;;c2) (c1';;c2')
+    ...and so on.  
 
-    We will see a concrete example of why these congruence properties
-    are important in the following section (in the proof of
-    [fold_constants_com_sound]), but the main idea is that they allow
-    us to replace a small part of a large program with an equivalent
-    small part and know that the whole large programs are equivalent
-    _without_ doing an explicit proof about the non-varying parts --
-    i.e., the "proof burden" of a small change to a large program is
-    proportional to the size of the change, not the program. *)
+    (Note that we are using the inference rule notation here not as
+    part of a definition, but simply to write down some valid
+    implications in a readable format. We prove these implications
+    below.) *)
 (** よりわかりにくいですが、振る舞い同値は、合同関係(_congruence_)でもあります。
     つまり、2つのサブプログラムが同値ならば、それを含むプログラム全体も同値です:
 [[
@@ -831,9 +824,18 @@ Proof.
     ...などです。
     (注意して欲しいのですが、ここで推論規則の記法を使っていますが、これは定義の一部ではありません。
     単に正しい含意を読みやすい形で書き出しただけです。
-    この含意は以下で証明します。)
+    この含意は以下で証明します。) *)
 
-    合同性がなぜ重要なのか、
+(*  We will see a concrete example of why these congruence
+    properties are important in the following section (in the proof of
+    [fold_constants_com_sound]), but the main idea is that they allow
+    us to replace a small part of a large program with an equivalent
+    small part and know that the whole large programs are equivalent
+    _without_ doing an explicit proof about the non-varying parts --
+    i.e., the "proof burden" of a small change to a large program is
+    proportional to the size of the change, not the program. *)
+
+(** 合同性がなぜ重要なのか、
     次の節で具体的な例([fold_constants_com_sound]の証明)によって見ます。
     ただ、メインのアイデアは、大きなプログラムの小さな部分を同値の小さな部分で置き換えると、
     大きなプログラム全体が元のものと同値になることを、
@@ -848,13 +850,13 @@ Proof.
   intros i a1 a2 Heqv st st'.
   split; intros Hceval.
   Case "->".
-    inversion Hceval. subst. apply E_Ass.
+    inversion Hceval. subst. apply E_Ass. 
     rewrite Heqv. reflexivity.
   Case "<-".
     inversion Hceval. subst. apply E_Ass.
     rewrite Heqv. reflexivity.  Qed.
 
-(* The congruence property for loops is a little more interesting,
+(** The congruence property for loops is a little more interesting,
     since it requires induction.
 
     _Theorem_: Equivalence is a congruence for [WHILE] -- that is, if
@@ -882,7 +884,7 @@ Proof.
             b1 = true], with [c1 / st || st'0] and [WHILE b1 DO c1
             END / st'0 || st'] for some state [st'0], with the
             induction hypothesis [WHILE b1' DO c1' END / st'0 ||
-            st'].
+            st'].  
 
             Since [c1] and [c1'] are equivalent, we know that [c1' /
             st || st'0].  And since [b1] and [b1'] are equivalent, we
@@ -933,31 +935,32 @@ Theorem CWhile_congruence : forall b1 b1' c1 c1',
   bequiv b1 b1' -> cequiv c1 c1' ->
   cequiv (WHILE b1 DO c1 END) (WHILE b1' DO c1' END).
 Proof.
+  (* WORKED IN CLASS *)
   unfold bequiv,cequiv.
   intros b1 b1' c1 c1' Hb1e Hc1e st st'.
   split; intros Hce.
   Case "->".
-    remember (WHILE b1 DO c1 END) as cwhile.
+    remember (WHILE b1 DO c1 END) as cwhile eqn:Heqcwhile.
     induction Hce; inversion Heqcwhile; subst.
     SCase "E_WhileEnd".
       apply E_WhileEnd. rewrite <- Hb1e. apply H.
     SCase "E_WhileLoop".
       apply E_WhileLoop with (st' := st').
       SSCase "show loop runs". rewrite <- Hb1e. apply H.
-      SSCase "body execution".
-        apply (Hc1e st st').  apply Hce1.
+      SSCase "body execution". 
+        apply (Hc1e st st').  apply Hce1. 
       SSCase "subsequent loop execution".
         apply IHHce2. reflexivity.
   Case "<-".
-    remember (WHILE b1' DO c1' END) as c'while.
+    remember (WHILE b1' DO c1' END) as c'while eqn:Heqc'while.
     induction Hce; inversion Heqc'while; subst.
     SCase "E_WhileEnd".
       apply E_WhileEnd. rewrite -> Hb1e. apply H.
     SCase "E_WhileLoop".
       apply E_WhileLoop with (st' := st').
       SSCase "show loop runs". rewrite -> Hb1e. apply H.
-      SSCase "body execution".
-        apply (Hc1e st st').  apply Hce1.
+      SSCase "body execution". 
+        apply (Hc1e st st').  apply Hce1. 
       SSCase "subsequent loop execution".
         apply IHHce2. reflexivity.  Qed.
 
@@ -965,8 +968,8 @@ Proof.
 (** **** 練習問題: ★★★, optional (CSeq_congruence) *)
 Theorem CSeq_congruence : forall c1 c1' c2 c2',
   cequiv c1 c1' -> cequiv c2 c2' ->
-  cequiv (c1;c2) (c1';c2').
-Proof.
+  cequiv (c1;;c2) (c1';;c2').
+Proof. 
   (* FILL IN HERE *) Admitted.
 (** [] *)
 
@@ -979,20 +982,24 @@ Proof.
   (* FILL IN HERE *) Admitted.
 (** [] *)
 
-(* For example, here are two equivalent programs and a proof of their
+(** *** *)
+
+(*  For example, here are two equivalent programs and a proof of their
     equivalence... *)
 (** 同値である2つのプログラムとその同値の証明の例です... *)
 
 Example congruence_example:
   cequiv
-    (X ::= ANum 0;
+    (* Program 1: *)
+    (X ::= ANum 0;;
      IFB (BEq (AId X) (ANum 0))
      THEN
        Y ::= ANum 0
      ELSE
        Y ::= ANum 42
      FI)
-    (X ::= ANum 0;
+    (* Program 2: *)
+    (X ::= ANum 0;;
      IFB (BEq (AId X) (ANum 0))
      THEN
        Y ::= AMinus (AId X) (AId X)   (* <--- changed here *)
@@ -1000,18 +1007,18 @@ Example congruence_example:
        Y ::= ANum 42
      FI).
 Proof.
-  apply CSeq_congruence.
-    apply refl_cequiv.
+  apply CSeq_congruence. 
+    apply refl_cequiv. 
     apply CIf_congruence.
       apply refl_bequiv.
-      apply CAss_congruence. unfold aequiv. simpl.
+      apply CAss_congruence. unfold aequiv. simpl. 
         symmetry. apply minus_diag.
-      apply refl_cequiv.
+      apply refl_cequiv. 
 Qed.
 
 (* ####################################################### *)
-(* * Case Study: Constant Folding *)
-(** * ケーススタディ: 定数畳み込み *)
+(*  * Program Transformations *)
+(** プログラムの変換 *)
 
 (* A _program transformation_ is a function that takes a program
     as input and produces some variant of the program as its
@@ -1021,13 +1028,9 @@ Qed.
     プログラムを入力とし、出力としてそのプログラムの何らかの変形を生成する関数です。
     定数畳み込みのようなコンパイラの最適化は標準的な例ですが、それ以外のものもたくさんあります。*)
 
-(* ####################################################### *)
-(* ** Soundness of Program Transformations *)
-(** ** プログラム変換の健全性 *)
-
 (* A program transformation is _sound_ if it preserves the
-    behavior of the original program.
-
+    behavior of the original program. 
+ 
     We can define a notion of soundness for translations of
     [aexp]s, [bexp]s, and [com]s. *)
 (** プログラム変換が健全(_sound_)とは、その変換が元のプログラムの振る舞いを保存することです。
@@ -1063,17 +1066,17 @@ Fixpoint fold_constants_aexp (a : aexp) : aexp :=
   match a with
   | ANum n       => ANum n
   | AId i        => AId i
-  | APlus a1 a2  =>
+  | APlus a1 a2  => 
       match (fold_constants_aexp a1, fold_constants_aexp a2) with
       | (ANum n1, ANum n2) => ANum (n1 + n2)
       | (a1', a2') => APlus a1' a2'
       end
-  | AMinus a1 a2 =>
+  | AMinus a1 a2 => 
       match (fold_constants_aexp a1, fold_constants_aexp a2) with
       | (ANum n1, ANum n2) => ANum (n1 - n2)
       | (a1', a2') => AMinus a1' a2'
       end
-  | AMult a1 a2  =>
+  | AMult a1 a2  => 
       match (fold_constants_aexp a1, fold_constants_aexp a2) with
       | (ANum n1, ANum n2) => ANum (n1 * n2)
       | (a1', a2') => AMult a1' a2'
@@ -1081,8 +1084,8 @@ Fixpoint fold_constants_aexp (a : aexp) : aexp :=
   end.
 
 Example fold_aexp_ex1 :
-    fold_constants_aexp
-      (AMult (APlus (ANum 1) (ANum 2)) (AId X))
+    fold_constants_aexp 
+      (AMult (APlus (ANum 1) (ANum 2)) (AId X)) 
   = AMult (ANum 3) (AId X).
 Proof. reflexivity. Qed.
 
@@ -1097,12 +1100,13 @@ Proof. reflexivity. Qed.
     定義と証明が長くなるだけです。*)
 
 Example fold_aexp_ex2 :
-    fold_constants_aexp
+    fold_constants_aexp 
       (AMinus (AId X) (APlus (AMult (ANum 0) (ANum 6)) (AId Y)))
   = AMinus (AId X) (APlus (ANum 0) (AId Y)).
 Proof. reflexivity. Qed.
 
-(* Not only can we lift [fold_constants_aexp] to [bexp]s (in the
+(** *** *)
+(*  Not only can we lift [fold_constants_aexp] to [bexp]s (in the
     [BEq] and [BLe] cases), we can also find constant _boolean_
     expressions and reduce them in-place. *)
 (** ([BEq]と[BLe]の場合に)[fold_constants_aexp]を[bexp]
@@ -1112,23 +1116,23 @@ Fixpoint fold_constants_bexp (b : bexp) : bexp :=
   match b with
   | BTrue        => BTrue
   | BFalse       => BFalse
-  | BEq a1 a2  =>
+  | BEq a1 a2  => 
       match (fold_constants_aexp a1, fold_constants_aexp a2) with
       | (ANum n1, ANum n2) => if beq_nat n1 n2 then BTrue else BFalse
       | (a1', a2') => BEq a1' a2'
       end
-  | BLe a1 a2  =>
+  | BLe a1 a2  => 
       match (fold_constants_aexp a1, fold_constants_aexp a2) with
       | (ANum n1, ANum n2) => if ble_nat n1 n2 then BTrue else BFalse
       | (a1', a2') => BLe a1' a2'
       end
-  | BNot b1  =>
+  | BNot b1  => 
       match (fold_constants_bexp b1) with
       | BTrue => BFalse
       | BFalse => BTrue
       | b1' => BNot b1'
       end
-  | BAnd b1 b2  =>
+  | BAnd b1 b2  => 
       match (fold_constants_bexp b1, fold_constants_bexp b2) with
       | (BTrue, BTrue) => BTrue
       | (BTrue, BFalse) => BFalse
@@ -1144,33 +1148,34 @@ Example fold_bexp_ex1 :
 Proof. reflexivity. Qed.
 
 Example fold_bexp_ex2 :
-    fold_constants_bexp
-      (BAnd (BEq (AId X) (AId Y))
-            (BEq (ANum 0)
+    fold_constants_bexp 
+      (BAnd (BEq (AId X) (AId Y)) 
+            (BEq (ANum 0) 
                  (AMinus (ANum 2) (APlus (ANum 1) (ANum 1)))))
   = BAnd (BEq (AId X) (AId Y)) BTrue.
 Proof. reflexivity. Qed.
 
-(* To fold constants in a command, we apply the appropriate folding
+(** *** *)
+(*  To fold constants in a command, we apply the appropriate folding
     functions on all embedded expressions. *)
 (** コマンド内の定数を畳み込みするために、含まれるすべての式に対応する畳み込み関数を適用します。*)
 
 Fixpoint fold_constants_com (c : com) : com :=
   match c with
-  | SKIP      =>
+  | SKIP      => 
       SKIP
-  | i ::= a  =>
+  | i ::= a  => 
       CAss i (fold_constants_aexp a)
-  | c1 ; c2  =>
-      (fold_constants_com c1) ; (fold_constants_com c2)
-  | IFB b THEN c1 ELSE c2 FI =>
+  | c1 ;; c2  => 
+      (fold_constants_com c1) ;; (fold_constants_com c2)
+  | IFB b THEN c1 ELSE c2 FI => 
       match fold_constants_bexp b with
       | BTrue => fold_constants_com c1
       | BFalse => fold_constants_com c2
-      | b' => IFB b' THEN fold_constants_com c1
+      | b' => IFB b' THEN fold_constants_com c1 
                      ELSE fold_constants_com c2 FI
       end
-  | WHILE b DO c END =>
+  | WHILE b DO c END => 
       match fold_constants_bexp b with
       | BTrue => WHILE BTrue DO SKIP END
       | BFalse => SKIP
@@ -1178,44 +1183,48 @@ Fixpoint fold_constants_com (c : com) : com :=
       end
   end.
 
+(** *** *)
 Example fold_com_ex1 :
-  fold_constants_com
-    (X ::= APlus (ANum 4) (ANum 5);
-     Y ::= AMinus (AId X) (ANum 3);
+  fold_constants_com 
+    (* Original program: *)
+    (X ::= APlus (ANum 4) (ANum 5);;
+     Y ::= AMinus (AId X) (ANum 3);;
      IFB BEq (AMinus (AId X) (AId Y)) (APlus (ANum 2) (ANum 4)) THEN
-       SKIP
+       SKIP 
      ELSE
        Y ::= ANum 0
-     FI;
+     FI;;
      IFB BLe (ANum 0) (AMinus (ANum 4) (APlus (ANum 2) (ANum 1))) THEN
        Y ::= ANum 0
      ELSE
-       SKIP
-     FI;
-     WHILE BEq (AId Y) (ANum 0) DO
-       X ::= APlus (AId X) (ANum 1)
-     END) =
-  (X ::= ANum 9;
-   Y ::= AMinus (AId X) (ANum 3);
-   IFB BEq (AMinus (AId X) (AId Y)) (ANum 6) THEN
-     SKIP
-   ELSE
-     (Y ::= ANum 0)
-   FI;
-   Y ::= ANum 0;
-   WHILE BEq (AId Y) (ANum 0) DO
-     X ::= APlus (AId X) (ANum 1)
-   END).
+       SKIP 
+     FI;;
+     WHILE BEq (AId Y) (ANum 0) DO 
+       X ::= APlus (AId X) (ANum 1) 
+     END) 
+  = (* After constant folding: *)
+    (X ::= ANum 9;;
+     Y ::= AMinus (AId X) (ANum 3);;
+     IFB BEq (AMinus (AId X) (AId Y)) (ANum 6) THEN
+       SKIP 
+     ELSE
+       (Y ::= ANum 0) 
+     FI;;
+     Y ::= ANum 0;;
+     WHILE BEq (AId Y) (ANum 0) DO 
+       X ::= APlus (AId X) (ANum 1) 
+     END).
 Proof. reflexivity. Qed.
 
 (* ################################################### *)
 (* ** Soundness of Constant Folding *)
 (** ** 定数畳み込みの健全性 *)
 
-(* Now we need to show that what we've done is correct.  Here's
-    the proof for arithmetic expressions: *)
-(** 上でやったことが正しいことを示さなければなりません。以下が算術式に対する証明です: *)
+(* Now we need to show that what we've done is correct. *)
+(** 上でやったことが正しいことを示さなければなりません。*)
 
+(*  Here's the proof for arithmetic expressions: *)
+(** 算術式に対する証明です: *)
 Theorem fold_constants_aexp_sound :
   atrans_sound fold_constants_aexp.
 Proof.
@@ -1225,15 +1234,15 @@ Proof.
     try reflexivity;
     (* APlus, AMinus, and AMult follow from the IH
        and the observation that
-              aeval st (APlus a1 a2)
-            = ANum ((aeval st a1) + (aeval st a2))
+              aeval st (APlus a1 a2) 
+            = ANum ((aeval st a1) + (aeval st a2)) 
             = aeval st (ANum ((aeval st a1) + (aeval st a2)))
        (and similarly for AMinus/minus and AMult/mult) *)
     try (destruct (fold_constants_aexp a1);
          destruct (fold_constants_aexp a2);
          rewrite IHa1; rewrite IHa2; reflexivity). Qed.
 
-(* **** Exercise: 3 stars, optional (fold_bexp_BEq_informal) *)
+(* **** Exercise: 3 stars, optional (fold_bexp_BEq_informal)  *)
 (** **** 練習問題: ★★★, optional (fold_bexp_BEq_informal) *)
 (* Here is an informal proof of the [BEq] case of the soundness
     argument for boolean expression constant folding.  Read it
@@ -1248,83 +1257,62 @@ Proof.
    for all boolean expressions [b].  Proceed by induction on [b].  We
    show just the case where [b] has the form [BEq a1 a2].
 
-   In this case, we must show
-[[
-       beval st (BEq a1 a2)
+   In this case, we must show 
+       beval st (BEq a1 a2) 
      = beval st (fold_constants_bexp (BEq a1 a2)).
-]]
    There are two cases to consider:
 
      - First, suppose [fold_constants_aexp a1 = ANum n1] and
        [fold_constants_aexp a2 = ANum n2] for some [n1] and [n2].
 
        In this case, we have
-[[
-           fold_constants_bexp (BEq a1 a2)
+           fold_constants_bexp (BEq a1 a2) 
          = if beq_nat n1 n2 then BTrue else BFalse
-]]
        and
-[[
-           beval st (BEq a1 a2)
+           beval st (BEq a1 a2) 
          = beq_nat (aeval st a1) (aeval st a2).
-]]
        By the soundness of constant folding for arithmetic
        expressions (Lemma [fold_constants_aexp_sound]), we know
-[[
-           aeval st a1
-         = aeval st (fold_constants_aexp a1)
-         = aeval st (ANum n1)
+           aeval st a1 
+         = aeval st (fold_constants_aexp a1) 
+         = aeval st (ANum n1) 
          = n1
-]]
        and
-[[
-           aeval st a2
-         = aeval st (fold_constants_aexp a2)
-         = aeval st (ANum n2)
+           aeval st a2 
+         = aeval st (fold_constants_aexp a2) 
+         = aeval st (ANum n2) 
          = n2,
-]]
        so
-[[
-           beval st (BEq a1 a2)
+           beval st (BEq a1 a2) 
          = beq_nat (aeval a1) (aeval a2)
          = beq_nat n1 n2.
-]]
        Also, it is easy to see (by considering the cases [n1 = n2] and
        [n1 <> n2] separately) that
-[[
            beval st (if beq_nat n1 n2 then BTrue else BFalse)
          = if beq_nat n1 n2 then beval st BTrue else beval st BFalse
          = if beq_nat n1 n2 then true else false
          = beq_nat n1 n2.
-]]
        So
-[[
-           beval st (BEq a1 a2)
+           beval st (BEq a1 a2) 
          = beq_nat n1 n2.
          = beval st (if beq_nat n1 n2 then BTrue else BFalse),
-]]
+]]         
        as required.
 
      - Otherwise, one of [fold_constants_aexp a1] and
        [fold_constants_aexp a2] is not a constant.  In this case, we
        must show
-[[
-           beval st (BEq a1 a2)
+           beval st (BEq a1 a2) 
          = beval st (BEq (fold_constants_aexp a1)
                          (fold_constants_aexp a2)),
-]]
        which, by the definition of [beval], is the same as showing
-[[
-           beq_nat (aeval st a1) (aeval st a2)
+           beq_nat (aeval st a1) (aeval st a2) 
          = beq_nat (aeval st (fold_constants_aexp a1))
                    (aeval st (fold_constants_aexp a2)).
-]]
        But the soundness of constant folding for arithmetic
        expressions ([fold_constants_aexp_sound]) gives us
-[[
          aeval st a1 = aeval st (fold_constants_aexp a1)
          aeval st a2 = aeval st (fold_constants_aexp a2),
-]]
        completing the case.  []
 *)
 (** ここに、ブール式の定数畳み込みに関する健全性の議論の[BEq]の場合の非形式的証明を示します。
@@ -1339,83 +1327,61 @@ Proof.
    [b]が[BEq a1 a2]という形の場合を示す。
 
    この場合、
-[[
        beval st (BEq a1 a2)
      = beval st (fold_constants_bexp (BEq a1 a2)).
-]]
    を示せば良い。これには2種類の場合がある:
 
      - 最初に、ある[n1]と[n2]について、[fold_constants_aexp a1 = ANum n1]かつ
        [fold_constants_aexp a2 = ANum n2]と仮定する。
 
        この場合、
-[[
            fold_constants_bexp (BEq a1 a2)
          = if beq_nat n1 n2 then BTrue else BFalse
-]]
        かつ
-[[
            beval st (BEq a1 a2)
          = beq_nat (aeval st a1) (aeval st a2).
-]]
        となる。
        算術式についての定数畳み込みの健全性(補題[fold_constants_aexp_sound])より、
-[[
            aeval st a1
          = aeval st (fold_constants_aexp a1)
          = aeval st (ANum n1)
          = n1
-]]
        かつ
-[[
            aeval st a2
          = aeval st (fold_constants_aexp a2)
          = aeval st (ANum n2)
          = n2,
-]]
        である。
        従って、
-[[
            beval st (BEq a1 a2)
          = beq_nat (aeval a1) (aeval a2)
          = beq_nat n1 n2.
-]]
        となる。また、([n1 = n2]と[n1 <> n2]の場合をそれぞれ考えると)
-[[
            beval st (if beq_nat n1 n2 then BTrue else BFalse)
          = if beq_nat n1 n2 then beval st BTrue else beval st BFalse
          = if beq_nat n1 n2 then true else false
          = beq_nat n1 n2.
-]]
        となることは明らかである。
        ゆえに
-[[
            beval st (BEq a1 a2)
          = beq_nat n1 n2.
          = beval st (if beq_nat n1 n2 then BTrue else BFalse),
-]]
        となる。これは求められる性質である。
 
      - それ以外の場合、[fold_constants_aexp a1]と[fold_constants_aexp a2]
        のどちらかは定数ではない。この場合、
-[[
            beval st (BEq a1 a2)
          = beval st (BEq (fold_constants_aexp a1)
                          (fold_constants_aexp a2)),
-]]
        を示せば良い。
        [beval]の定義から、これは     
-[[
            beq_nat (aeval st a1) (aeval st a2)
          = beq_nat (aeval st (fold_constants_aexp a1))
                    (aeval st (fold_constants_aexp a2)).
-]]
        を示すことと同じである。
        算術式についての定数畳み込みの健全性([fold_constants_aexp_sound])より、
-[[
          aeval st a1 = aeval st (fold_constants_aexp a1)
          aeval st a2 = aeval st (fold_constants_aexp a2),
-]]
        となり、この場合も成立する。[]
 *)
 
@@ -1423,36 +1389,36 @@ Theorem fold_constants_bexp_sound:
   btrans_sound fold_constants_bexp.
 Proof.
   unfold btrans_sound. intros b. unfold bequiv. intros st.
-  bexp_cases (induction b) Case;
+  bexp_cases (induction b) Case; 
     (* BTrue and BFalse are immediate *)
-    try reflexivity.
-  Case "BEq".
+    try reflexivity. 
+  Case "BEq". 
     (* Doing induction when there are a lot of constructors makes
        specifying variable names a chore, but Coq doesn't always
        choose nice variable names.  We can rename entries in the
        context with the [rename] tactic: [rename a into a1] will
        change [a] to [a1] in the current goal and context. *)
     rename a into a1. rename a0 into a2. simpl.
-    remember (fold_constants_aexp a1) as a1'.
-    remember (fold_constants_aexp a2) as a2'.
+    remember (fold_constants_aexp a1) as a1' eqn:Heqa1'.
+    remember (fold_constants_aexp a2) as a2' eqn:Heqa2'.
     replace (aeval st a1) with (aeval st a1') by
        (subst a1'; rewrite <- fold_constants_aexp_sound; reflexivity).
     replace (aeval st a2) with (aeval st a2') by
        (subst a2'; rewrite <- fold_constants_aexp_sound; reflexivity).
     destruct a1'; destruct a2'; try reflexivity.
-      (* The only interesting case is when both a1 and a2
+      (* The only interesting case is when both a1 and a2 
          become constants after folding *)
       simpl. destruct (beq_nat n n0); reflexivity.
-  Case "BLe".
+  Case "BLe". 
     (* FILL IN HERE *) admit.
-  Case "BNot".
-    simpl. remember (fold_constants_bexp b) as b'.
+  Case "BNot". 
+    simpl. remember (fold_constants_bexp b) as b' eqn:Heqb'. 
     rewrite IHb.
-    destruct b'; reflexivity.
-  Case "BAnd".
-    simpl.
-    remember (fold_constants_bexp b1) as b1'.
-    remember (fold_constants_bexp b2) as b2'.
+    destruct b'; reflexivity. 
+  Case "BAnd". 
+    simpl. 
+    remember (fold_constants_bexp b1) as b1' eqn:Heqb1'. 
+    remember (fold_constants_bexp b2) as b2' eqn:Heqb2'.
     rewrite IHb1. rewrite IHb2.
     destruct b1'; destruct b2'; reflexivity.  Qed.
 (** [] *)
@@ -1462,19 +1428,18 @@ Proof.
 (* Complete the [WHILE] case of the following proof. *)
 (** 次の証明の[WHILE]の場合を完成させなさい。*)
 
-Theorem fold_constants_com_sound :
+Theorem fold_constants_com_sound : 
   ctrans_sound fold_constants_com.
-Proof.
-  unfold ctrans_sound. intros c.
+Proof. 
+  unfold ctrans_sound. intros c. 
   com_cases (induction c) Case; simpl.
   Case "SKIP". apply refl_cequiv.
   Case "::=". apply CAss_congruence. apply fold_constants_aexp_sound.
-  Case ";". apply CSeq_congruence; assumption.
-  Case "IFB".
+  Case ";;". apply CSeq_congruence; assumption.
+  Case "IFB". 
     assert (bequiv b (fold_constants_bexp b)).
       SCase "Pf of assertion". apply fold_constants_bexp_sound.
-    remember (fold_constants_bexp b) as b'.
-    destruct b';
+    destruct (fold_constants_bexp b) eqn:Heqb;
       (* If the optimization doesn't eliminate the if, then the result
          is easy to prove from the IH and fold_constants_bexp_sound *)
       try (apply CIf_congruence; assumption).
@@ -1495,34 +1460,30 @@ Proof.
 (* **** Exercise: 4 stars, optional (optimize_0plus) *)
 (** **** 練習問題: ★★★★, optional (optimize_0plus) *)
 (* Recall the definition [optimize_0plus] from Imp.v:
-[[
     Fixpoint optimize_0plus (e:aexp) : aexp :=
       match e with
-      | ANum n =>
+      | ANum n => 
           ANum n
-      | APlus (ANum 0) e2 =>
+      | APlus (ANum 0) e2 => 
           optimize_0plus e2
-      | APlus e1 e2 =>
+      | APlus e1 e2 => 
           APlus (optimize_0plus e1) (optimize_0plus e2)
-      | AMinus e1 e2 =>
+      | AMinus e1 e2 => 
           AMinus (optimize_0plus e1) (optimize_0plus e2)
-      | AMult e1 e2 =>
+      | AMult e1 e2 => 
           AMult (optimize_0plus e1) (optimize_0plus e2)
       end.
-]]
    Note that this function is defined over the old [aexp]s,
    without states.
 
    Write a new version of this function that accounts for variables,
    and analogous ones for [bexp]s and commands:
-[[
      optimize_0plus_aexp
      optimize_0plus_bexp
      optimize_0plus_com
-]]
    Prove that these three functions are sound, as we did for
-   [fold_constants_*].  Make sure you use the congruence lemmas in
-   the proof of [optimize_0plus_com] (otherwise it will be _long_!).
+   [fold_constants_*].  (Make sure you use the congruence lemmas in
+   the proof of [optimize_0plus_com] -- otherwise it will be _long_!)
 
    Then define an optimizer on commands that first folds
    constants (using [fold_constants_com]) and then eliminates [0 + n]
@@ -1533,21 +1494,19 @@ Proof.
    - Prove that the optimizer is sound.  (This part should be _very_
      easy.)  *)
 (** Imp_J.vの[optimize_0plus]の定義をふり返ります。
-[[
     Fixpoint optimize_0plus (e:aexp) : aexp :=
       match e with
-      | ANum n =>
+      | ANum n => 
           ANum n
-      | APlus (ANum 0) e2 =>
+      | APlus (ANum 0) e2 => 
           optimize_0plus e2
-      | APlus e1 e2 =>
+      | APlus e1 e2 => 
           APlus (optimize_0plus e1) (optimize_0plus e2)
-      | AMinus e1 e2 =>
+      | AMinus e1 e2 => 
           AMinus (optimize_0plus e1) (optimize_0plus e2)
-      | AMult e1 e2 =>
+      | AMult e1 e2 => 
           AMult (optimize_0plus e1) (optimize_0plus e2)
       end.
-]]
    この関数は、[aexp]の上で定義されていて、状態を扱わないことに注意します。
 
    変数を扱えるようにした、この関数の新しいバージョンを記述しなさい。
@@ -1580,34 +1539,29 @@ Proof.
     and [c2] is the command [X ::= a1; Y ::= a2'], where [a2'] is
     formed by substituting [a1] for all occurrences of [X] in [a2].
     For example, [c1] and [c2] might be:
-[[
-       c1  =  (X ::= 42 + 53;
+       c1  =  (X ::= 42 + 53;; 
                Y ::= Y + X)
-       c2  =  (X ::= 42 + 53;
+       c2  =  (X ::= 42 + 53;; 
                Y ::= Y + (42 + 53))
-]]
-    Clearly, this particular [c1] and [c2] are equivalent.  But is
-    this true in general? *)
+    Clearly, this _particular_ [c1] and [c2] are equivalent.  Is this
+    true in general? *)
 (** [c1]が[X ::= a1; Y ::= a2]という形のコマンドで、
     [c2]がコマンド[X ::= a1; Y ::= a2']であると仮定します。ただし[a2']は、
     [a2]の中のすべてのXを[a1]で置換したものとします。
     例えば、[c1]と[c2]は次のようなものです。
-[[
        c1  =  (X ::= 42 + 53;
                Y ::= Y + X)
-       c2  =  (X ::= 42 + 53;
+       c2  =  (X ::= 42 + 53;; 
                Y ::= Y + (42 + 53))
-]]
     明らかに、この例の場合は[c1]と[c2]は同値です。
     しかし、一般にそうだと言えるでしょうか？ *)
 
-(* We will see in a moment that it is not, but it is worthwhile
+(*  We will see in a moment that it is not, but it is worthwhile
     to pause, now, and see if you can find a counter-example on your
-    own (or remember the one from the discussion in class). *)
+    own. *)
 (** この後すぐ、そうではないことを示します。
     しかし、ここでちょっと立ち止まって、
-    自分の力で反例を見つけることができるか試してみるのは意味があることです。
-    (あるいは、クラスでの議論を思い出してください。) *)
+    自分の力で反例を見つけることができるか試してみるのは意味があることです。 *)
 
 (* Here, formally, is the function that substitutes an arithmetic
     expression for each occurrence of a given variable in another
@@ -1617,7 +1571,7 @@ Proof.
 Fixpoint subst_aexp (i : id) (u : aexp) (a : aexp) : aexp :=
   match a with
   | ANum n       => ANum n
-  | AId i'       => if beq_id i i' then u else AId i'
+  | AId i'       => if eq_id_dec i i' then u else AId i'
   | APlus a1 a2  => APlus (subst_aexp i u a1) (subst_aexp i u a2)
   | AMinus a1 a2 => AMinus (subst_aexp i u a1) (subst_aexp i u a2)
   | AMult a1 a2  => AMult (subst_aexp i u a1) (subst_aexp i u a2)
@@ -1635,95 +1589,72 @@ Proof. reflexivity.  Qed.
     上記コマンド[c1]と[c2]が常に同値であることを主張するものです。*)
 
 Definition subst_equiv_property := forall i1 i2 a1 a2,
-  cequiv (i1 ::= a1; i2 ::= a2)
-         (i1 ::= a1; i2 ::= subst_aexp i1 a1 a2).
+  cequiv (i1 ::= a1;; i2 ::= a2)
+         (i1 ::= a1;; i2 ::= subst_aexp i1 a1 a2).
 
-(* Sadly, the property does _not_ always hold.
+(** *** *)
+(*  Sadly, the property does _not_ always hold. 
 
     _Theorem_: It is not the case that, for all [i1], [i2], [a1],
     and [a2],
-[[
-         cequiv (i1 ::= a1; i2 ::= a2)
-                (i1 ::= a1; i2 ::= subst_aexp i1 a1 a2).
-]]
+         cequiv (i1 ::= a1;; i2 ::= a2)
+                (i1 ::= a1;; i2 ::= subst_aexp i1 a1 a2).
+]] 
     _Proof_: Suppose, for a contradiction, that for all [i1], [i2],
     [a1], and [a2], we have
-[[
-      cequiv (i1 ::= a1; i2 ::= a2)
-             (i1 ::= a1; i2 ::= subst_aexp i1 a1 a2).
-]]
+      cequiv (i1 ::= a1;; i2 ::= a2) 
+             (i1 ::= a1;; i2 ::= subst_aexp i1 a1 a2).
     Consider the following program:
-[[
-         X ::= APlus (AId X) (ANum 1); Y ::= AId X
-]]
+         X ::= APlus (AId X) (ANum 1);; Y ::= AId X
     Note that
-[[
-         (X ::= APlus (AId X) (ANum 1); Y ::= AId X)
+         (X ::= APlus (AId X) (ANum 1);; Y ::= AId X)
          / empty_state || st1,
-]]
     where [st1 = { X |-> 1, Y |-> 1 }].
 
     By our assumption, we know that
-[[
-        cequiv (X ::= APlus (AId X) (ANum 1); Y ::= AId X)
-               (X ::= APlus (AId X) (ANum 1); Y ::= APlus (AId X) (ANum 1))
-]]
+        cequiv (X ::= APlus (AId X) (ANum 1);; Y ::= AId X)
+               (X ::= APlus (AId X) (ANum 1);; Y ::= APlus (AId X) (ANum 1))
     so, by the definition of [cequiv], we have
-[[
-        (X ::= APlus (AId X) (ANum 1); Y ::= APlus (AId X) (ANum 1))
+        (X ::= APlus (AId X) (ANum 1);; Y ::= APlus (AId X) (ANum 1))
         / empty_state || st1.
-]]
     But we can also derive
-[[
-        (X ::= APlus (AId X) (ANum 1); Y ::= APlus (AId X) (ANum 1))
+        (X ::= APlus (AId X) (ANum 1);; Y ::= APlus (AId X) (ANum 1))
         / empty_state || st2,
-]]
     where [st2 = { X |-> 1, Y |-> 2 }].  Note that [st1 <> st2]; this
     is a contradiction, since [ceval] is deterministic!  [] *)
 (** 残念ながら、この性質は、常には成立「しません」。
 
     「定理」:すべての[i1], [i2], [a1], [a2]について、次が成立するわけではない:
-[[
-         cequiv (i1 ::= a1; i2 ::= a2)
-                (i1 ::= a1; i2 ::= subst_aexp i1 a1 a2).
+
+         cequiv (i1 ::= a1;; i2 ::= a2)
+                (i1 ::= a1;; i2 ::= subst_aexp i1 a1 a2).
 ]]
+
     「証明」:仮にすべての[i1], [i2], [a1], [a2]について
-[[
-      cequiv (i1 ::= a1; i2 ::= a2)
-             (i1 ::= a1; i2 ::= subst_aexp i1 a1 a2)
-]]
+      cequiv (i1 ::= a1;; i2 ::= a2) 
+             (i1 ::= a1;; i2 ::= subst_aexp i1 a1 a2).
     が成立するとする。
     次のプログラムを考える:
-[[
-         X ::= APlus (AId X) (ANum 1); Y ::= AId X
-]]
+         X ::= APlus (AId X) (ANum 1);; Y ::= AId X
     次のことに注意する:
-[[
-         (X ::= APlus (AId X) (ANum 1); Y ::= AId X)
+         (X ::= APlus (AId X) (ANum 1);; Y ::= AId X)
          / empty_state || st1,
-]]
     ここで [st1 = { X |-> 1, Y |-> 1 }]である。
 
     仮定より、次が言える:
-[[
-        cequiv (X ::= APlus (AId X) (ANum 1); Y ::= AId X)
-               (X ::= APlus (AId X) (ANum 1); Y ::= APlus (AId X) (ANum 1))
-]]
+        cequiv (X ::= APlus (AId X) (ANum 1);; Y ::= AId X)
+               (X ::= APlus (AId X) (ANum 1);; Y ::= APlus (AId X) (ANum 1))
     すると、[cequiv]の定義より、次が言える:
-[[
-        (X ::= APlus (AId X) (ANum 1); Y ::= APlus (AId X) (ANum 1))
+        (X ::= APlus (AId X) (ANum 1);; Y ::= APlus (AId X) (ANum 1))
         / empty_state || st1.
-]]
     しかし次のことも言える:
-[[
-        (X ::= APlus (AId X) (ANum 1); Y ::= APlus (AId X) (ANum 1))
+        (X ::= APlus (AId X) (ANum 1);; Y ::= APlus (AId X) (ANum 1))
         / empty_state || st2,
-]]
     ただし[st2 = { X |-> 1, Y |-> 2 }]である。
     [st1 <> st2]に注意すると、これは[ceval]が決定性を持つことに矛盾する!
       [] *)
 
-Theorem subst_inequiv :
+Theorem subst_inequiv : 
   ~ subst_equiv_property.
 Proof.
   unfold subst_equiv_property.
@@ -1801,13 +1732,268 @@ Proof.
 (* FILL IN HERE *)
 (** [] *)
 
-(* **** Exercise: 3 stars, recommended (inequiv_exercise) *)
-(** **** 練習問題: ★★★, recommended (inequiv_exercise) *)
-Theorem inequiv_exercise:
+(* **** Exercise: 3 stars, recommended (inequiv_exercise)  *)
+(** **** 練習問題: ★★★, recommended (inequiv_exercise)  *)
+(*  Prove that an infinite loop is not equivalent to [SKIP] *)
+(** 無限ループは、[SKIP]と等しくないことを証明しなさい *)
+Theorem inequiv_exercise: 
   ~ cequiv (WHILE BTrue DO SKIP END) SKIP.
 Proof.
   (* FILL IN HERE *) Admitted.
 (** [] *)
+
+(** * Extended exercise: Non-deterministic Imp *)
+
+(** As we have seen (in theorem [ceval_deterministic] in the Imp
+    chapter), Imp's evaluation relation is deterministic.  However,
+    _non_-determinism is an important part of the definition of many
+    real programming languages. For example, in many imperative
+    languages (such as C and its relatives), the order in which
+    function arguments are evaluated is unspecified.  The program
+    fragment
+      x = 0;;
+      f(++x, x)
+    might call [f] with arguments [(1, 0)] or [(1, 1)], depending how
+    the compiler chooses to order things.  This can be a little
+    confusing for programmers, but it gives the compiler writer useful
+    freedom.
+
+    In this exercise, we will extend Imp with a simple
+    non-deterministic command and study how this change affects
+    program equivalence.  The new command has the syntax [HAVOC X],
+    where [X] is an identifier. The effect of executing [HAVOC X] is
+    to assign an _arbitrary_ number to the variable [X],
+    non-deterministically. For example, after executing the program:
+      HAVOC Y;;
+      Z ::= Y * 2
+    the value of [Y] can be any number, while the value of [Z] is
+    twice that of [Y] (so [Z] is always even). Note that we are not
+    saying anything about the _probabilities_ of the outcomes -- just
+    that there are (infinitely) many different outcomes that can
+    possibly happen after executing this non-deterministic code.
+
+    In a sense a variable on which we do [HAVOC] roughly corresponds
+    to an unitialized variable in the C programming language. After
+    the [HAVOC] the variable holds a fixed but arbitrary number.  Most
+    sources of nondeterminism in language definitions are there
+    precisely because programmers don't care which choice is made (and
+    so it is good to leave it open to the compiler to choose whichever
+    will run faster).
+
+    We call this new language _Himp_ (``Imp extended with [HAVOC]''). *)
+
+Module Himp.
+
+(** To formalize the language, we first add a clause to the definition of
+   commands. *)
+
+Inductive com : Type :=
+  | CSkip : com
+  | CAss : id -> aexp -> com
+  | CSeq : com -> com -> com
+  | CIf : bexp -> com -> com -> com
+  | CWhile : bexp -> com -> com
+  | CHavoc : id -> com.                (* <---- new *)
+
+Tactic Notation "com_cases" tactic(first) ident(c) :=
+  first;
+  [ Case_aux c "SKIP" | Case_aux c "::=" | Case_aux c ";;"
+  | Case_aux c "IFB" | Case_aux c "WHILE" | Case_aux c "HAVOC" ].
+
+Notation "'SKIP'" :=
+  CSkip.
+Notation "X '::=' a" :=
+  (CAss X a) (at level 60).
+Notation "c1 ;; c2" :=
+  (CSeq c1 c2) (at level 80, right associativity).
+Notation "'WHILE' b 'DO' c 'END'" :=
+  (CWhile b c) (at level 80, right associativity).
+Notation "'IFB' e1 'THEN' e2 'ELSE' e3 'FI'" :=
+  (CIf e1 e2 e3) (at level 80, right associativity).
+Notation "'HAVOC' l" := (CHavoc l) (at level 60).
+
+(** **** Exercise: 2 stars (himp_ceval)  *)
+(** Now, we must extend the operational semantics. We have provided
+   a template for the [ceval] relation below, specifying the big-step
+   semantics. What rule(s) must be added to the definition of [ceval]
+   to formalize the behavior of the [HAVOC] command? *)
+
+Reserved Notation "c1 '/' st '||' st'" (at level 40, st at level 39).
+
+Inductive ceval : com -> state -> state -> Prop :=
+  | E_Skip : forall st : state, SKIP / st || st
+  | E_Ass : forall (st : state) (a1 : aexp) (n : nat) (X : id),
+            aeval st a1 = n -> (X ::= a1) / st || update st X n
+  | E_Seq : forall (c1 c2 : com) (st st' st'' : state),
+            c1 / st || st' -> c2 / st' || st'' -> (c1 ;; c2) / st || st''
+  | E_IfTrue : forall (st st' : state) (b1 : bexp) (c1 c2 : com),
+               beval st b1 = true ->
+               c1 / st || st' -> (IFB b1 THEN c1 ELSE c2 FI) / st || st'
+  | E_IfFalse : forall (st st' : state) (b1 : bexp) (c1 c2 : com),
+                beval st b1 = false ->
+                c2 / st || st' -> (IFB b1 THEN c1 ELSE c2 FI) / st || st'
+  | E_WhileEnd : forall (b1 : bexp) (st : state) (c1 : com),
+                 beval st b1 = false -> (WHILE b1 DO c1 END) / st || st
+  | E_WhileLoop : forall (st st' st'' : state) (b1 : bexp) (c1 : com),
+                  beval st b1 = true ->
+                  c1 / st || st' ->
+                  (WHILE b1 DO c1 END) / st' || st'' ->
+                  (WHILE b1 DO c1 END) / st || st''
+(* FILL IN HERE *)
+
+  where "c1 '/' st '||' st'" := (ceval c1 st st').
+
+Tactic Notation "ceval_cases" tactic(first) ident(c) :=
+  first;
+  [ Case_aux c "E_Skip" | Case_aux c "E_Ass" | Case_aux c "E_Seq"
+  | Case_aux c "E_IfTrue" | Case_aux c "E_IfFalse"
+  | Case_aux c "E_WhileEnd" | Case_aux c "E_WhileLoop"
+(* FILL IN HERE *)
+].
+
+(** As a sanity check, the following claims should be provable for
+   your definition: *)
+
+Example havoc_example1 : (HAVOC X) / empty_state || update empty_state X 0.
+Proof.
+(* FILL IN HERE *) Admitted.
+
+Example havoc_example2 :
+  (SKIP;; HAVOC Z) / empty_state || update empty_state Z 42.
+Proof.
+(* FILL IN HERE *) Admitted.
+(** [] *)
+
+(** Finally, we repeat the definition of command equivalence from above: *)
+
+Definition cequiv (c1 c2 : com) : Prop := forall st st' : state,
+  c1 / st || st' <-> c2 / st || st'.
+
+(** This definition still makes perfect sense in the case of always
+    terminating programs, so let's apply it to prove some
+    non-deterministic programs equivalent or non-equivalent. *)
+
+(** **** Exercise: 3 stars (havoc_swap)  *)
+(** Are the following two programs equivalent? *)
+
+Definition pXY :=
+  HAVOC X;; HAVOC Y.
+
+Definition pYX :=
+  HAVOC Y;; HAVOC X.
+
+(** If you think they are equivalent, prove it. If you think they are
+    not, prove that. *)
+
+
+Theorem pXY_cequiv_pYX :
+  cequiv pXY pYX \/ ~cequiv pXY pYX.
+Proof. (* FILL IN HERE *) Admitted.
+(** [] *)
+
+(** **** Exercise: 4 stars, optional (havoc_copy)  *)
+(** Are the following two programs equivalent? *)
+
+Definition ptwice :=
+  HAVOC X;; HAVOC Y.
+
+Definition pcopy :=
+  HAVOC X;; Y ::= AId X.
+
+(** If you think they are equivalent, then prove it. If you think they
+    are not, then prove that.  (Hint: You may find the [assert] tactic
+    useful.) *)
+
+Theorem ptwice_cequiv_pcopy :
+  cequiv ptwice pcopy \/ ~cequiv ptwice pcopy.
+Proof. (* FILL IN HERE *) Admitted.
+(** [] *)
+
+(** The definition of program equivalence we are using here has some
+    subtle consequences on programs that may loop forever.  What
+    [cequiv] says is that the set of possible _terminating_ outcomes
+    of two equivalent programs is the same. However, in a language
+    with non-determinism, like Himp, some programs always terminate,
+    some programs always diverge, and some programs can
+    non-deterministically terminate in some runs and diverge in
+    others. The final part of the following exercise illustrates this
+    phenomenon.
+*)
+
+(** **** Exercise: 5 stars, advanced (p1_p2_equiv)  *)
+(** Prove that p1 and p2 are equivalent. In this and the following
+    exercises, try to understand why the [cequiv] definition has the
+    behavior it has on these examples. *)
+
+Definition p1 : com :=
+  WHILE (BNot (BEq (AId X) (ANum 0))) DO
+    HAVOC Y;;
+    X ::= APlus (AId X) (ANum 1)
+  END.
+
+Definition p2 : com :=
+  WHILE (BNot (BEq (AId X) (ANum 0))) DO
+    SKIP
+  END.
+
+
+(** Intuitively, the programs have the same termination
+    behavior: either they loop forever, or they terminate in the
+    same state they started in.  We can capture the termination
+    behavior of p1 and p2 individually with these lemmas: *)
+
+Lemma p1_may_diverge : forall st st', st X <> 0 ->
+  ~ p1 / st || st'.
+Proof. (* FILL IN HERE *) Admitted.
+
+Lemma p2_may_diverge : forall st st', st X <> 0 ->
+  ~ p2 / st || st'.
+Proof.
+(* FILL IN HERE *) Admitted.
+
+(** You should use these lemmas to prove that p1 and p2 are actually
+    equivalent. *)
+
+Theorem p1_p2_equiv : cequiv p1 p2.
+Proof. (* FILL IN HERE *) Admitted.
+(** [] *)
+
+(** **** Exercise: 4 stars, advanced (p3_p4_inquiv)  *)
+
+(** Prove that the following programs are _not_ equivalent. *)
+
+Definition p3 : com :=
+  Z ::= ANum 1;;
+  WHILE (BNot (BEq (AId X) (ANum 0))) DO
+    HAVOC X;;
+    HAVOC Z
+  END.
+
+Definition p4 : com :=
+  X ::= (ANum 0);;
+  Z ::= (ANum 1).
+
+
+Theorem p3_p4_inequiv : ~ cequiv p3 p4.
+Proof. (* FILL IN HERE *) Admitted.
+(** [] *)
+
+(** **** Exercise: 5 stars, advanced, optional (p5_p6_equiv)  *)
+
+Definition p5 : com :=
+  WHILE (BNot (BEq (AId X) (ANum 1))) DO
+    HAVOC X
+  END.
+
+Definition p6 : com :=
+  X ::= ANum 1.
+
+
+Theorem p5_p6_equiv : cequiv p5 p6.
+Proof. (* FILL IN HERE *) Admitted.
+(** [] *)
+
+End Himp.
 
 (* ####################################################### *)
 (* * Doing Without Extensionality (Optional) *)
@@ -1871,11 +2057,11 @@ Proof.
 
 (* **** Exercise: 1 star, optional (stequiv_trans) *)
 (** **** 練習問題: ★, optional (stequiv_trans) *)
-Lemma stequiv_trans : forall (st1 st2 st3 : state),
-  st1 ~ st2 ->
-  st2 ~ st3 ->
+Lemma stequiv_trans : forall (st1 st2 st3 : state), 
+  st1 ~ st2 -> 
+  st2 ~ st3 -> 
   st1 ~ st3.
-Proof.
+Proof.  
   (* FILL IN HERE *) Admitted.
 (** [] *)
 
@@ -1884,9 +2070,9 @@ Proof.
 (* **** Exercise: 1 star, optional (stequiv_update) *)
 (** **** 練習問題: ★, optional (stequiv_update) *)
 Lemma stequiv_update : forall (st1 st2 : state),
-  st1 ~ st2 ->
+  st1 ~ st2 -> 
   forall (X:id) (n:nat),
-  update st1 X n ~ update st2 X n.
+  update st1 X n ~ update st2 X n. 
 Proof.
   (* FILL IN HERE *) Admitted.
 (** [] *)
@@ -1898,18 +2084,18 @@ Proof.
 
 (* **** Exercise: 2 stars, optional (stequiv_aeval) *)
 (** **** 練習問題: ★★, optional (stequiv_aeval) *)
-Lemma stequiv_aeval : forall (st1 st2 : state),
+Lemma stequiv_aeval : forall (st1 st2 : state), 
   st1 ~ st2 ->
-  forall (a:aexp), aeval st1 a = aeval st2 a.
+  forall (a:aexp), aeval st1 a = aeval st2 a. 
 Proof.
   (* FILL IN HERE *) Admitted.
 (** [] *)
 
 (* **** Exercise: 2 stars, optional (stequiv_beval) *)
 (** **** 練習問題: ★★, optional (stequiv_beval) *)
-Lemma stequiv_beval : forall (st1 st2 : state),
+Lemma stequiv_beval : forall (st1 st2 : state), 
   st1 ~ st2 ->
-  forall (b:bexp), beval st1 b = beval st2 b.
+  forall (b:bexp), beval st1 b = beval st2 b. 
 Proof.
   (* FILL IN HERE *) Admitted.
 (** [] *)
@@ -1927,41 +2113,41 @@ Lemma stequiv_ceval: forall (st1 st2 : state),
     exists st2' : state,
     ((c / st2 || st2') /\  st1' ~ st2').
 Proof.
-  intros st1 st2 STEQV c st1' CEV1. generalize dependent st2.
-  induction CEV1; intros st2 STEQV.
+  intros st1 st2 STEQV c st1' CEV1. generalize dependent st2. 
+  induction CEV1; intros st2 STEQV.  
   Case "SKIP".
-    exists st2. split.
-      constructor.
+    exists st2. split.  
+      constructor. 
       assumption.
   Case ":=".
-    exists (update st2 l n). split.
-       constructor.  rewrite <- H. symmetry.  apply stequiv_aeval.
+    exists (update st2 x n). split. 
+       constructor.  rewrite <- H. symmetry.  apply stequiv_aeval. 
        assumption. apply stequiv_update.  assumption.
   Case ";".
     destruct (IHCEV1_1 st2 STEQV) as [st2' [P1 EQV1]].
-    destruct (IHCEV1_2 st2' EQV1) as [st2'' [P2 EQV2]].
+    destruct (IHCEV1_2 st2' EQV1) as [st2'' [P2 EQV2]]. 
     exists st2''.  split.
-      apply E_Seq with st2';  assumption.
+      apply E_Seq with st2';  assumption. 
       assumption.
   Case "IfTrue".
     destruct (IHCEV1 st2 STEQV) as [st2' [P EQV]].
-    exists st2'.  split.
-      apply E_IfTrue.  rewrite <- H. symmetry. apply stequiv_beval.
+    exists st2'.  split. 
+      apply E_IfTrue.  rewrite <- H. symmetry. apply stequiv_beval. 
       assumption. assumption. assumption.
   Case "IfFalse".
     destruct (IHCEV1 st2 STEQV) as [st2' [P EQV]].
-    exists st2'. split.
-     apply E_IfFalse. rewrite <- H. symmetry. apply stequiv_beval.
+    exists st2'. split. 
+     apply E_IfFalse. rewrite <- H. symmetry. apply stequiv_beval. 
      assumption.  assumption. assumption.
   Case "WhileEnd".
     exists st2. split.
-      apply E_WhileEnd. rewrite <- H. symmetry. apply stequiv_beval.
-      assumption. assumption.
+      apply E_WhileEnd. rewrite <- H. symmetry. apply stequiv_beval. 
+      assumption. assumption. 
   Case "WhileLoop".
     destruct (IHCEV1_1 st2 STEQV) as [st2' [P1 EQV1]].
     destruct (IHCEV1_2 st2' EQV1) as [st2'' [P2 EQV2]].
-    exists st2''. split.
-      apply E_WhileLoop with st2'.  rewrite <- H. symmetry.
+    exists st2''. split. 
+      apply E_WhileLoop with st2'.  rewrite <- H. symmetry. 
       apply stequiv_beval. assumption. assumption. assumption.
       assumption.
 Qed.
@@ -1981,7 +2167,7 @@ Reserved Notation "c1 '/' st '||'' st'" (at level 40, st at level 39).
 
 Inductive ceval' : com -> state -> state -> Prop :=
   | E_equiv : forall c st st' st'',
-    c / st || st' ->
+    c / st || st' -> 
     st' ~ st'' ->
     c / st ||' st''
   where   "c1 '/' st '||'' st'" := (ceval' c1 st st').
@@ -2001,11 +2187,11 @@ Definition cequiv' (c1 c2 : com) : Prop :=
 
 Lemma cequiv__cequiv' : forall (c1 c2: com),
   cequiv c1 c2 -> cequiv' c1 c2.
-Proof.
-  unfold cequiv, cequiv'; split; intros.
-    inversion H0 ; subst.  apply E_equiv with st'0.
-    apply (H st st'0); assumption. assumption.
-    inversion H0 ; subst.  apply E_equiv with st'0.
+Proof. 
+  unfold cequiv, cequiv'; split; intros. 
+    inversion H0 ; subst.  apply E_equiv with st'0.  
+    apply (H st st'0); assumption. assumption. 
+    inversion H0 ; subst.  apply E_equiv with st'0.  
     apply (H st st'0). assumption. assumption.
 Qed.
 
@@ -2018,14 +2204,14 @@ Qed.
 Example identity_assignment' :
   cequiv' SKIP (X ::= AId X).
 Proof.
-    unfold cequiv'.  intros.  split; intros.
+    unfold cequiv'.  intros.  split; intros. 
     Case "->".
-      inversion H; subst; clear H. inversion H0; subst.
-      apply E_equiv with (update st'0 X (st'0 X)).
-      constructor. reflexivity.  apply stequiv_trans with st'0.
-      unfold stequiv. intros. apply update_same.
-      reflexivity. assumption.
-    Case "<-".
+      inversion H; subst; clear H. inversion H0; subst.   
+      apply E_equiv with (update st'0 X (st'0 X)). 
+      constructor. reflexivity.  apply stequiv_trans with st'0.  
+      unfold stequiv. intros. apply update_same. 
+      reflexivity. assumption. 
+    Case "<-".  
       (* FILL IN HERE *) Admitted.
 (** [] *)
 
@@ -2060,37 +2246,29 @@ Proof.
 (* This exercise extends the optional add_for_loop exercise from
     Imp.v, where you were asked to extend the language of commands
     with C-style [for] loops.  Prove that the command:
-[[
       for (c1 ; b ; c2) {
           c3
       }
-]]
     is equivalent to:
-[[
-       c1 ;
+       c1 ; 
        WHILE b DO
          c3 ;
          c2
        END
-]]
 *)
 (** この練習問題は、Imp_J.vのoptionalの練習問題 add_for_loop を拡張したものです。
     もとの add_for_loop は、コマンド言語に C-言語のスタイルの [for]ループを
     拡張しなさい、というものでした。
     ここでは次のことを証明しなさい:    
-[[
       for (c1 ; b ; c2) {
           c3
       }
-]]
     は
-[[
        c1 ;
        WHILE b DO
          c3 ;
          c2
        END
-]]
     と同値である。
 *)
 (* FILL IN HERE *)
@@ -2099,13 +2277,13 @@ Proof.
 (* **** Exercise: 3 stars, optional (swap_noninterfering_assignments) *)
 (** **** 練習問題: ★★★, optional (swap_noninterfering_assignments) *)
 Theorem swap_noninterfering_assignments: forall l1 l2 a1 a2,
-  l1 <> l2 ->
+  l1 <> l2 -> 
   var_not_used_in_aexp l1 a2 ->
   var_not_used_in_aexp l2 a1 ->
   cequiv
-    (l1 ::= a1; l2 ::= a2)
-    (l2 ::= a2; l1 ::= a1).
-Proof.
+    (l1 ::= a1;; l2 ::= a2)
+    (l2 ::= a2;; l1 ::= a1).
+Proof. 
 (* Hint: You'll need [functional_extensionality] *)
 (* ヒント: [functional_extensionality]を必要とするでしょう。 *)
 (* FILL IN HERE *) Admitted.
